Clap/eDSLState/Varstore.lean
@@ -6,11 +6,22 @@ namespace Clap
 def VarStore (p : ℕ) := Std.ExtTreeMap ℕ (ZMod p) (cmp := compare)
 deriving Inhabited, Repr
 
+def VarStore.contains {p : ℕ} (Γ : VarStore p) (x : ℕ) : Bool := Std.ExtTreeMap.contains Γ x
+
 instance {p : ℕ} : EmptyCollection (VarStore p) := inferInstanceAs (EmptyCollection (Std.ExtTreeMap ℕ (ZMod p)))
 
-instance {p : ℕ} : GetElem? (VarStore p) ℕ (ZMod p) (λ Γ x ↦ Γ.contains x) where
+instance instVarStoreGetElem? {p : ℕ} : GetElem? (VarStore p) ℕ (ZMod p) (λ (Γ : VarStore p) x ↦ Γ.contains x) where
   getElem  Γ x h := Γ.get x h
   getElem? Γ x   := Γ.get? x
+
+instance {p : ℕ} : LawfulGetElem (VarStore p) ℕ (ZMod p) (λ (Γ : VarStore p) x ↦ Γ.contains x) where
+  getElem?_def Γ x inst := by
+    have : LawfulGetElem (Std.ExtTreeMap ℕ (ZMod p)) ℕ (ZMod p) (λ m x ↦ m.contains x) := inferInstance
+    obtain ⟨h_getElem, _⟩ := this
+    specialize h_getElem Γ x
+    unfold VarStore.contains
+    unfold_projs at h_getElem ⊢
+    convert h_getElem
 
 instance {p : ℕ} : HasSubset (VarStore p) where
   Subset Γ1 Γ2 := ∀ k : ℕ, Γ1[k]?.isSome → Γ1[k]? = Γ2[k]?
